{
 "cells": [
  {
   "cell_type": "markdown",
   "id": "eaab649d",
   "metadata": {},
   "source": [
    "### Roll No. ME22MTECH14006\n",
    "### Name. Aman Gautam\n",
    "### Assignment 1  "
   ]
  },
  {
   "cell_type": "markdown",
   "id": "090032e1",
   "metadata": {},
   "source": [
    "#### Question 1\n",
    "\n",
    "(a)\n",
    "\n",
    "i.) \n",
    "\n",
    "Cross-Product\n",
    "\n",
    "$a \\times b = a_ib_j\\epsilon_{ijk}\\mathbf{e}_k$\n",
    "\n",
    "Dot-Product\n",
    "\n",
    "$a \\cdot b = a_ib_j$\n",
    "\n",
    "ii.)\n",
    "\n",
    "LHS :\n",
    "\n",
    "$A_{ij}\\delta_{jk}$\n",
    "\n",
    "$A_{ij}e_j \\cdot e_k$\n",
    "\n",
    "\n",
    "This expression is 0 for j!=k. Thus we will chose j = k for with kronekar delta is 1 and we get the following\n",
    "\n",
    "$A_{ik}$ = RHS.\n",
    "\n",
    "or we put values of repeating index\n",
    "\n",
    "LHS = $A_{i1}\\delta_{1k} + A_{i2}\\delta_{2k} + A_{i3}\\delta_{3k}$\n",
    "\n",
    "Similar to previous argument $\\delta_{ij}$ vanishes if $i != j$ thus when $k$ assumes value (1,2,3) only the corresponding term survives, That is\n",
    "\n",
    "$k = 1$\n",
    "\n",
    "LHS = $A_{i1}\\delta_{11} + A_{i2}\\delta_{21} + A_{i3}\\delta_{31} = A_{i1}$\n",
    "\n",
    "$k = 2$\n",
    "\n",
    "LHS = $A_{i2}\\delta_{12} + A_{i2}\\delta_{22} + A_{i3}\\delta_{32} = A_{i2}$\n",
    "\n",
    "$k = 3$\n",
    "\n",
    "LHS = $A_{i1}\\delta_{13} + A_{i2}\\delta_{23} + A_{i3}\\delta_{33} = A_{i3}$\n",
    "\n",
    "this shows that\n",
    "\n",
    "LHS = $A_{ik}$ which is equal to RHS\n",
    "\n",
    "Hence Proved\n",
    "\n",
    "iii.) \n",
    "\n",
    "$\\delta_{ij}\\delta_{ij}  = \\delta_{ii} = \\delta_{11} + \\delta_{22} + \\delta_{33} = 1 + 1 + 1 = 3$\n",
    "\n",
    "\n",
    "---\n",
    "\n",
    "(b)\n",
    "\n",
    "Given \n",
    "\n",
    "$T_{ij} = \\lambda E_{kk} \\delta_{ij} + 2 \\mu E_{ij}$\n",
    "\n",
    "\n",
    "i.) $W = \\frac{1}{2}T_{ij}E_{ij}$\n",
    "\n",
    "Substituting values\n",
    "\n",
    "$W = \\frac{1}{2}(\\lambda E_{kk} \\delta_{ij} + 2 \\mu E_{ij})E_{ij}$\n",
    "\n",
    "$W = \\frac{1}{2}(\\lambda E_{kk}E_{jj} + 2 \\mu E_{ij}E_{ij})$\n",
    "\n",
    "$W = \\frac{1}{2}\\lambda E_{kk}^2 + \\mu E_{ij}E_{ij}$\n",
    "\n",
    "\n",
    "ii.) $P = T_{ij}T_{ij}$\n",
    "\n",
    "$P = (\\lambda E_{kk} \\delta_{ij} + 2 \\mu E_{ij})(\\lambda E_{pp} \\delta_{ij} + 2 \\mu E_{ij})$\n",
    "\n",
    "$P = \\lambda^2 E_{kk}E_{pp} \\delta_{ij}\\delta_{ij} + 2 \\mu E_{ij} \\lambda E_{pp} \\delta_{ij} + 2 \\mu E_{ij} \\lambda E_{kk} \\delta_{ij} + 4 \\mu^2 E_{ij}E_{ij} $\n",
    "\n",
    "$P = 3\\lambda^2 E_{kk}E_{pp}  + 2 \\mu E_{jj} \\lambda E_{pp}  + 2 \\mu E_{jj} \\lambda E_{kk}  + 4 \\mu^2 E_{ij}E_{ij} $\n",
    "\n",
    "$P = 3\\lambda^2 E_{kk}^2  + 4 \\mu\\lambda E_{jj}^2  + 4 \\mu^2 E_{ij}E_{ij} $\n",
    "\n",
    "$P = 3\\lambda^2 E_{kk}^2  + 4 \\mu\\lambda E_{kk}^2  + 4 \\mu^2 E_{ij}E_{ij} $  (Traces are equal $A_{ii} = A_{jj}$)\n",
    "\n",
    "$P = \\lambda E_{kk}^2(3\\lambda  + 4 \\mu)  + 4 \\mu^2 E_{ij}E_{ij} $   This is what we intended to show\n",
    "\n",
    "---\n",
    "\n",
    "(c) \n",
    "\n",
    "i.)\n",
    "\n",
    "$T'_{ij} = Q_{ki}T_{kp}Q_{pj}$  (This is how 2nd order tensors transform)\n",
    "\n",
    "Now we need to find value of $T'_{ii}$ for that we do $i == j$\n",
    "\n",
    "$T'_{ii} = Q_{ki}T_{kp}Q_{pi}$ \n",
    "\n",
    "$T'_{ii} = Q_{ki}Q_{pi}T_{kp}$\n",
    "\n",
    "Obserbe that $Q_{ki}Q_{pi}$ is actually $QQ^T$ which is equal to identity. Thus $Q_{ki}Q_{pi} = \\delta_{kp}$\n",
    "\n",
    "$T'_{ii} = \\delta_{kp}T_{kp}$\n",
    "\n",
    "Using property of Kronekar delta\n",
    "\n",
    "$T'_{ii} = T_{kk}$ This is what we intended to show\n",
    "\n",
    "\n",
    "ii.)\n",
    "\n",
    "$T'_{ij}T'_{ji} = trace(T'T')$\n",
    "\n",
    "$trace(T'T') = trace(Q^TTQQ^TTQ)$\n",
    "\n",
    "$trace(T'T') = trace(Q^TTTQ)$\n",
    "\n",
    "since $trace((AB)^T) = trace(AB)$ we can write\n",
    "\n",
    "$trace(Q^TTTQ) = tr)$\n",
    "\n",
    "\n",
    "iii.) \n",
    "\n",
    "Use the fact that determinant of Q is identity\n",
    "\n",
    "$det(T'_{ij}) = det(T') = det(Q^TTQ) = det(Q)det(T)det(Q) = det(T)$ \n",
    "\n",
    "\n",
    "---\n",
    "\n",
    "(d) and (e) part in code cell below"
   ]
  },
  {
   "cell_type": "code",
   "execution_count": 4,
   "id": "aabd3ed8",
   "metadata": {},
   "outputs": [],
   "source": [
    "'''\n",
    "d part of question 1\n",
    "'''\n",
    "\n",
    "import numpy as np\n",
    "\n",
    "def kdelta(i,j):\n",
    "    return int(i == j)\n",
    "\n",
    "def GetIndex(i,j):\n",
    "    flag = int(((10*i+j) in [21,2,10]))\n",
    "    if(i == j):\n",
    "        a = i\n",
    "    else:\n",
    "        a = 6 - j - i + 3*flag\n",
    "    return a,flag\n",
    "\n",
    "def Get2DMatrixFormOf4thOrderTensor(C):\n",
    "    '''\n",
    "    This convertes general 4th order tensor to 2D 9x9 matrix representation\n",
    "    For major and minor symmetries only first 6 rows and colums survive giving 4th order elasticity tensor\n",
    "    '''\n",
    "    C_1 = np.zeros((9,9))\n",
    "    for i in range(3):\n",
    "        for j in range(3):\n",
    "            a, f1 = GetIndex(i, j)\n",
    "            for k in range(3):\n",
    "                for l in range(3):\n",
    "                    b,f2 = GetIndex(k,l)\n",
    "                    C_1[a][b] = 0.25*(C[i][j][k][l] + (-1)**(f1)*C[j][i][k][l] + \n",
    "                                      (-1)**(f2)*C[i][j][l][k] + (-1)**(f2)*(-1)**(f1)*C[j][i][l][k])\n",
    "    return C_1\n",
    "\n",
    "\n",
    "'''\n",
    "(e)\n",
    "Following 2 functions generate 2nd and 4th order identity tensors\n",
    "'''\n",
    "\n",
    "def Get2DIdentity(n = 3):\n",
    "    return np.eye(n)\n",
    "\n",
    "def Get4DIdentity(n = 3):\n",
    "    I = np.zeros((n,n,n,n))\n",
    "    for i in range(n):\n",
    "        for j in range(n):\n",
    "            for k in range(n):\n",
    "                for l in range(n):\n",
    "                    I[i][j][k][l] = kdelta(i,j)*kdelta(k,l)\n",
    "    return I"
   ]
  },
  {
   "cell_type": "markdown",
   "id": "4b856895",
   "metadata": {},
   "source": [
    "#### Question 2\n",
    "\n",
    "$x_1 = \\frac{1}{4}(18 + 4x_1 + 6x_2)$\n",
    "\n",
    "$x_2 = \\frac{1}{4}(14 + 6x_2)$\n",
    "\n",
    "$x_3 = x_3$\n",
    "\n",
    "(a) \n",
    "\n"
   ]
  }
 ],
 "metadata": {
  "kernelspec": {
   "display_name": "Python 3 (ipykernel)",
   "language": "python",
   "name": "python3"
  },
  "language_info": {
   "codemirror_mode": {
    "name": "ipython",
    "version": 3
   },
   "file_extension": ".py",
   "mimetype": "text/x-python",
   "name": "python",
   "nbconvert_exporter": "python",
   "pygments_lexer": "ipython3",
   "version": "3.9.12"
  }
 },
 "nbformat": 4,
 "nbformat_minor": 5
}
